Added argument about denotation being a partial function

theories/Semantics/IMP/Denotational.v
@@ -13,6 +13,10 @@ Definition denotb (b : BExp) : State -> bool :=
 Inductive delta : Ensemble (State * State) :=
 | delta_intro : forall (sigma : State), delta (sigma, sigma).
 
+Lemma elem_of_delta: forall (sigma sigma' : State),
+    (sigma, sigma') ∈ delta <-> sigma = sigma'.
+Proof. by split; [inversion 1 | intros ->; constructor]. Qed.
+
 Inductive denot_asgn (x : nat) (a : AExp) : Ensemble (State * State) :=
 | dasgn_intro : forall sigma : State,
     denot_asgn x a (sigma, update sigma x (denota a sigma)).
@@ -22,6 +26,17 @@ Inductive fwd_relation_composition
 | relation_composition_intro : forall a b c : State,
     (a, b) ∈ R -> (b, c) ∈ Q -> fwd_relation_composition R Q (a, c).
 
+Lemma elem_of_fwd_relation_composition:
+    forall (R Q : Ensemble (State * State)) (sigma sigma' : State),
+    (sigma, sigma') ∈ fwd_relation_composition R Q
+      <->
+    exists (sigma'' : State), (sigma, sigma'') ∈ R /\ (sigma'', sigma') ∈ Q.
+Proof.
+    intros; split.
+    - by inversion 1; subst; eexists; split.
+    - by intros (? & ? & ?); econstructor.
+Qed.
+
 Inductive relation_selector (cond : State -> bool)
     (Then Else : Ensemble (State * State)) : Ensemble (State * State) :=
 | relation_selector_then : forall (sigma sigma' : State), cond sigma = true ->
@@ -30,9 +45,40 @@ Inductive relation_selector (cond : State -> bool)
     (sigma, sigma') ∈ Else -> relation_selector cond Then Else (sigma, sigma')
 .
 
+Lemma elem_of_relation_selector:
+    forall (cond : State -> bool) (Then Else : Ensemble (State * State))
+        (sigma sigma' : State),
+    (sigma, sigma') ∈ relation_selector cond Then Else
+      <->
+    (cond sigma = true /\ (sigma, sigma') ∈ Then)
+      \/
+    (cond sigma = false /\ (sigma, sigma') ∈ Else).
+Proof.
+    split.
+    - by inversion 1; subst; [left | right].
+    - intros [[]|[]].
+      + by apply relation_selector_then.
+      + by apply relation_selector_else.
+Qed.
+
 Definition while_step (cond : State -> bool)
     (body while: Ensemble (State * State)) : Ensemble (State * State) :=
     relation_selector cond (fwd_relation_composition body while) delta.
+
+Lemma elem_of_while_step (cond : State -> bool)
+    (body while: Ensemble (State * State)):
+    forall (sigma sigma' : State),
+    (sigma, sigma') ∈ while_step cond body while
+      <->
+    (cond sigma = false /\ sigma = sigma')
+      \/
+    (cond sigma = true /\ exists (sigma'' : State), (sigma, sigma'') ∈ body /\ (sigma'', sigma') ∈ while).
+Proof.
+    intros; unfold while_step.
+    rewrite elem_of_relation_selector, elem_of_delta, elem_of_fwd_relation_composition.
+    by split; intros [|]; [right | left | right | left].
+Qed.
+
 
 #[export] Instance while_step_proper (cond : State -> bool)
     (body : Ensemble (State * State)) : Proper ((⊆) ==> (⊆)) (while_step cond body).
@@ -97,4 +143,111 @@ Proof.
           by constructor; eapply bs_while_true.
         * inversion H2; subst.
           by constructor; eapply bs_while_false.
+Qed.
+
+Definition partial_function `(R : Ensemble (A * B)) :=
+    forall (a : A) (b1 b2 : B), (a, b1) ∈ R -> (a, b2) ∈ R -> b1 = b2.
+
+#[export] Instance partial_function_proper {A B} : Proper ((≡) ==> iff) (@partial_function A B).
+Proof.
+    by intros R Q Heqv; unfold partial_function; setoid_rewrite Heqv.
+Qed.
+
+Lemma pf_empty : forall (A B : Type), @partial_function A B ∅.
+Proof. by intros * a b1 b2 Hb2; inversion Hb2. Qed.
+
+Lemma pf_delta : partial_function delta.
+Proof.
+    intros sigma sigma' sigma'' H' H''.
+    by inversion H'; inversion H''; subst.
+Qed.
+
+Lemma pf_denot_asgn : forall (x : nat) (a : AExp),
+    partial_function (denot_asgn x a).
+Proof.
+    intros x a sigma sigma' sigma'' H' H''.
+    by inversion H'; inversion H''; subst.
+Qed.
+
+Lemma pf_fwd_relation_composition: forall (R Q : Ensemble (State * State)),
+    partial_function R -> partial_function Q ->
+    partial_function (fwd_relation_composition R Q).
+Proof.
+    intros R Q HR HQ sigma sigma' sigma'' H' H''.
+    inversion H'; inversion H''; subst.
+    rewrite (HR sigma b b0 H1 H5) in *.
+    by rewrite (HQ b0 sigma' sigma'' H2 H6).
+Qed.
+
+Lemma pf_relation_selector: forall (cond : State -> bool) (Then Else : Ensemble (State * State)),
+    partial_function Then -> partial_function Else ->
+    partial_function (relation_selector cond Then Else).
+Proof.
+    intros * HThen HElse sigma sigma' sigma'' H' H''.
+    inversion H'; subst.
+    - inversion H''; [| by rewrite H1 in *; discriminate].
+      by rewrite (HThen sigma sigma' sigma'' H2 H4).
+    - inversion H''; [by rewrite H1 in *; discriminate |].
+      by rewrite (HElse sigma sigma' sigma'' H2 H4).
+Qed.
+
+Lemma pf_while_step: forall (cond : State -> bool) (body while : Ensemble (State * State)),
+    partial_function body -> partial_function while ->
+    partial_function (while_step cond body while).
+Proof.
+    by intros; apply pf_relation_selector;
+      [apply pf_fwd_relation_composition | apply pf_delta].
+Qed.
+
+#[export] Instance while_step_continuous:
+    forall (cond : State -> bool) (body : Ensemble (State * State)),
+    Continuous (while_step cond body).
+Proof.
+    intros *; constructor; intros C (sigma, sigma').
+    rewrite elem_of_while_step.
+    setoid_rewrite elem_of_indexed_union; cbn.
+    setoid_rewrite elem_of_while_step.
+    split; [intros [[]|[? (sigma'' & Hbody & i & HCi)]] | intros [i [[]|[? (sigma'' & Hbody & HCi)]]]].
+    - by exists 0; left.
+    - by exists i; right; repeat esplit.
+    - by left.
+    - by right; repeat esplit.
+Qed.
+
+Lemma pf_ascending_chain:
+    forall (C : nat -> Ensemble (State * State)),
+        (forall (n : nat), partial_function (C n)) ->
+        ascending_chain C ->
+        partial_function (indexed_union C).
+Proof.
+    intros C Hpf Hchain sigma sigma' sigma''.
+    rewrite !elem_of_indexed_union.
+    intros [i' Hsigma'] [i'' Hsigma''].
+    apply (Hpf (max i' i'') sigma sigma' sigma'').
+    - eapply ascending_chain_skipping; [done | | done].
+      by lia.
+    - eapply ascending_chain_skipping; [done | | done].
+      by lia.
+Qed.
+
+Lemma pf_denot_while : forall (cond : State -> bool) (body : Ensemble (State * State)),
+    partial_function body ->
+    partial_function (lfp (while_step cond body)).
+Proof.
+    intros cond body Hbody.
+    rewrite kleene_knaster_tarski_lfp_equiv;
+      [| by typeclasses eauto | by apply Omega_continuous_klfp_fixpoint; typeclasses eauto].
+    apply pf_ascending_chain; [| by apply kleene_ascending_chain; typeclasses eauto].
+    induction n; cbn; [apply pf_empty |].
+    by apply pf_while_step.
+Qed.
+
+Lemma pf_denotc: forall (c : Cmd), partial_function (denotc c).
+Proof.
+    induction c.
+    - by apply pf_delta.
+    - by apply pf_denot_asgn.
+    - by apply pf_fwd_relation_composition.
+    - by apply pf_relation_selector.
+    - by apply pf_denot_while.
 Qed.
